
% !TEX TS-program = pdflatex
% !TEX encoding = UTF-8 Unicode

% This is a simple template for a LaTeX document using the "article" class.
% See "book", "report", "letter" for other types of document.

\documentclass[11pt]{article} % use larger type; default would be 10pt

\usepackage[utf8x]{inputenc} % set input encoding (not needed with XeLaTeX)
\usepackage[russian]{babel}


\setlength{\parskip}{1em}

\begin{document}
\begin{flushleft}


\Large\textbf{Вариант 1} \\
$ z_1 = \frac{sin 2\alpha + sin 5\alpha - sin 3\alpha}{cos \alpha + 1 - 2 sin^2 2\alpha} $ \\
\vspace{0.5\baselineskip}
$ z_2 = 2 sin\alpha $

\par

\Large\textbf{Вариант 2} \\
$ z_1 = \frac{sin 2\alpha + sin 5\alpha - sin 3\alpha}{cos \alpha - cos 3\alpha + cos 5\alpha} $ \\
\vspace{0.5\baselineskip}
$ z_2 = tg 3\alpha $

\par 

\Large\textbf{Вариант 3} \\
$ z_1 = \frac{sin\left(\frac{\pi}{2} + 3\alpha\right)}{1 - sin\left(3\alpha - \pi\right)} $ \\
\vspace{0.5\baselineskip}
$ z_2 = ctg\left(\frac{5}{4}\pi + \frac{3}{2}\alpha\right) $

\par

\Large\textbf{Вариант 4} \\
$ z_1 = \frac{1 - 2 sin^2 \alpha}{1 + sin 2\alpha} $ \\
\vspace{0.5\baselineskip}
$ z_2 = \frac{1 - tg\alpha}{1 + tg\alpha} $

\par

\Large\textbf{Вариант 5} \\
$ z_1 = \frac{sin 4\alpha}{1 + cos 4\alpha} \cdot \frac{cos 2\alpha}{1 + cos 2\alpha} $ \\
\vspace{0.5\baselineskip}
$ z_2 = ctg\left( \frac{3}{2}\pi - \alpha \right) $

\par

\Large\textbf{Вариант 6} \\
$ z_1 = \frac{sin\alpha + cos\left(2\beta - \alpha\right)}{cos\alpha - sin\left(2\beta - \alpha\right)} $ \\
\vspace{0.5\baselineskip}
$ z_2 = \frac{1 + sin 2\beta}{cos 2\beta} $ 

\par 

\Large\textbf{Вариант 7} \\
$ z_1 = \frac{cos\alpha + sin\alpha}{cos\alpha - sin\alpha} $ \\
\vspace{0.5\baselineskip}
$ z_2 = tg 2\alpha + sec 2\alpha $ 

\par 

\Large\textbf{Вариант 8} \\
$ z_1 = \frac{\sqrt{2b + 2\sqrt{b^2 - 4}}}{\sqrt{b^2 - 4} + b + 2} $ \\
\vspace{0.5\baselineskip}
$ z_2 = \frac{1}{\sqrt{b + 2}} $

\par

\Large\textbf{Вариант 9} \\
$ z_1 = \frac{x^2 + 2x - 3 + \left(x + 1\right)\sqrt{x^2 - 9}}{x^2 - 2x - 3 + \left(x - 1\right)\sqrt{x^2 - 9}} $ \\
\vspace{0.5\baselineskip}
$ z_2 = \sqrt{\frac{x + 3}{x - 3}} $

\par

\Large\textbf{Вариант 10} \\
$ z_1 = \frac{\sqrt{\left(3m + 2\right)^2 - 24m}}{3\sqrt{m} - \frac{2}{\sqrt{m}}} $ \\
\vspace{0.5\baselineskip}
$ z_2 = -\sqrt{m} $

\par

\Large\textbf{Вариант 11} \\
$ z_1 = \left( \frac{a + 2}{\sqrt{2a}} - \frac{a}{\sqrt{2a} + 2} + \frac{2}{a - \sqrt{2a}} \right) \cdot \frac{\sqrt{a} - \sqrt{2}}{a + 2} $ \\
\vspace{0.5\baselineskip}
$ z_2 = \frac{1}{\sqrt{a} + \sqrt{2}} $

\par

\Large\textbf{Вариант 12} \\
$ z_1 = \left( \frac{1 + a + a^2}{2a + a^2} + 2 - \frac{1 - a + a^2}{2a - a^2} \right)^{-1} \left(5 - 2a^2 \right)  $ \\
\vspace{0.5\baselineskip}
$ z_2 = \frac{4 - a^2}{2} $

\par

\Large\textbf{Вариант 13} \\
$ z_1 = \frac{\left(m - 1\right)\sqrt{m} - \left(n - 1\right)\sqrt{n}}{\sqrt{m^3 n} + nm + m^2 - m} $ \\
\vspace{0.5\baselineskip}
$ z_2 = \frac{\sqrt{m} - \sqrt{n}}{m} $

\end{flushleft}
\end{document}
